src/QL/FOL/coding.lean
@@ -1,4 +1,4 @@
-import QL.FOL.fol provability consistency
+import QL.FOL.uniform provability consistency
 
 universes u v
 
@@ -6,54 +6,32 @@ namespace fol
 open_locale logic_symbol
 variables (L : language.{u}) {m n : ℕ}
 
-inductive uniform_subterm  (n : ℕ) : Type u
-| uvar  {} : ℕ → uniform_subterm
-| var   {} : fin n → uniform_subterm
-| function : ∀ {k}, L.fn k → (fin k → uniform_subterm) → uniform_subterm
-
-inductive uniform_subformula : ℕ → Type u
-| verum    {n} : uniform_subformula n
-| relation {n} : ∀ {p}, L.pr p → (fin p → uniform_subterm L n) → uniform_subformula n
-| imply    {n} : uniform_subformula n → uniform_subformula n → uniform_subformula n
-| neg      {n} : uniform_subformula n → uniform_subformula n
-| fal      {n} : uniform_subformula (n + 1) → uniform_subformula n
-
 namespace uniform_subterm
 variables {L n}
-
-@[simp] def uvars : uniform_subterm L n → ℕ
-| (uvar x)       := x + 1
-| (var x)        := 0
-| (function f v) := ⨆ᶠ i, (v i).uvars
-
-@[simp] def to_subterm : ∀ t : uniform_subterm L n, t.uvars ≤ m → subterm L m n
-| (uvar x)       h := &⟨x, h⟩
-| (var x)        h := #x 
-| (@function L n k f v) h := subterm.function f (λ i, to_subterm (v i) (by { haveI: inhabited (fin k) := ⟨i⟩, simp at h, exact h i}))
 
 section encode
 variables (L n)
 
 def label := ℕ ⊕ fin n ⊕ Σ n, L.fn n
 
-def arity : label L n → Type
+def label_type : label L n → Type
 | (sum.inl n)                := empty
 | (sum.inr $ sum.inl n)      := empty
 | (sum.inr $ sum.inr ⟨k, f⟩) := fin k
 
 variables {L n}
 
-@[reducible] def W_to_subterm : W_type (arity L n) → uniform_subterm L n
+@[reducible] def W_to_subterm : W_type (label_type L n) → uniform_subterm L n
 | ⟨sum.inl x, _⟩                := uvar x
 | ⟨sum.inr $ sum.inl x, _⟩      := var x
 | ⟨sum.inr $ sum.inr ⟨k, f⟩, F⟩ := function f (λ x, W_to_subterm (F x))
 
-def subterm_to_W : uniform_subterm L n → W_type (arity L n)
-| (uvar x)       := ⟨sum.inl x, empty.rec _⟩
+def subterm_to_W : uniform_subterm L n → W_type (label_type L n)
+| &&x       := ⟨sum.inl x, empty.rec _⟩
 | (var x)        := ⟨sum.inr $ sum.inl x, empty.rec _⟩
 | (function f v) := ⟨sum.inr $ sum.inr ⟨_, f⟩, λ i, subterm_to_W (v i)⟩
 
-def formula_equiv_W : uniform_subterm L n ≃ W_type (arity L n) :=
+def formula_equiv_W : uniform_subterm L n ≃ W_type (label_type L n) :=
 { to_fun := subterm_to_W,
   inv_fun := W_to_subterm,
   left_inv := by intros p; induction p; simp[subterm_to_W, W_to_subterm, *],
@@ -62,12 +40,12 @@ def formula_equiv_W : uniform_subterm L n ≃ W_type (arity L n) :=
     { rcases a, simp[subterm_to_W, W_to_subterm], exact funext (by rintros ⟨⟩) },
     { simp[subterm_to_W, W_to_subterm, IH] } } }
 
-instance : Π i, fintype (arity L n i)
+instance : Π i, fintype (label_type L n i)
 | (sum.inl a)                := show fintype empty, from fintype.of_is_empty
 | (sum.inr $ sum.inl x)      := show fintype empty, from fintype.of_is_empty
 | (sum.inr $ sum.inr ⟨k, f⟩) := fin.fintype k
 
-instance : Π i, encodable (arity L n i)
+instance : Π i, encodable (label_type L n i)
 | (sum.inl a)                := show encodable empty, from is_empty.to_encodable
 | (sum.inr $ sum.inl x)      := show encodable empty, from is_empty.to_encodable
 | (sum.inr $ sum.inr ⟨k, f⟩) := fin.encodable k
@@ -76,7 +54,8 @@ variables [∀ k, encodable (L.fn k)]
 
 instance : encodable (label L n) := sum.encodable
 
-instance : encodable (uniform_subterm L n) := encodable.of_equiv (W_type (arity L n)) formula_equiv_W
+@[irreducible]
+instance : encodable (uniform_subterm L n) := encodable.of_equiv (W_type (label_type L n)) formula_equiv_W
 
 end encode
 
@@ -86,36 +65,19 @@ namespace subterm
 open uniform_subterm
 variables {L m n}
 
-@[simp] def to_uniform : subterm L m n → uniform_subterm L n
-| &x             := uniform_subterm.uvar x 
-| #x             := uniform_subterm.var x 
-| (function f v) := uniform_subterm.function f (λ i, (v i).to_uniform)
-
-@[simp] lemma to_uniform_mlift (t : subterm L m n) : t.mlift.to_uniform = t.to_uniform :=
-by induction t; simp*
-
-@[simp] lemma to_uniform_to_subterm (t : subterm L m n) (h) : t.to_uniform.to_subterm h = t :=
-by induction t; simp*
-
-@[simp] lemma to_subterm_to_uniform (t : uniform_subterm L n) (h : t.uvars ≤ m) : (t.to_subterm h).to_uniform = t :=
-by induction t; simp*
-
 section encode
 
 variables [∀ k, encodable (L.fn k)]
 
-def to_nat : subterm L m n → ℕ := λ t, encodable.encode t.to_uniform
+def to_nat : subterm L m n → ℕ := λ t, encodable.encode t.uniform
 
 variables (L m n)
 
 def of_nat : ℕ → option (subterm L m n) := λ i,
   let t := encodable.decode (uniform_subterm L n) i in
-  t.bind (λ t, if h : t.uvars ≤ m then some (t.to_subterm h) else none)
+  t.bind (λ t, if h : t.arity ≤ m then some (t.to_subterm h) else none)
 
 variables {L m n}
-
-@[simp] lemma subterm_uvars (t : subterm L m n) : t.to_uniform.uvars ≤ m :=
-by { induction t; simp*, case metavar : i { exact nat.succ_le_iff.mpr i.property } }
 
 @[simp] lemma to_nat_of_nat (t : subterm L m n) : of_nat L m n t.to_nat = some t :=
 by simp[to_nat, of_nat]
@@ -127,22 +89,17 @@ end encode
 
 end subterm
 
+namespace uniform_subterm
+variables {L n} [∀ k, encodable (L.fn k)]
+
+@[simp] lemma to_nat_to_subterm (t : uniform_subterm L n) {m} (h : t.arity ≤ m) :
+  (t.to_subterm h).to_nat = encodable.encode t :=
+by simp[subterm.to_nat]
+
+end uniform_subterm
+
 namespace uniform_subformula
 variables {L n}
-
-@[simp] def uvars : Π {n}, uniform_subformula L n → ℕ
-| n verum          := 0
-| n (relation r v) := ⨆ᶠ i, (v i).uvars
-| n (imply p q)    := max p.uvars q.uvars
-| n (neg p)        := p.uvars
-| n (fal p)        := p.uvars
-
-@[simp] def to_subformula : ∀ {n} (p : uniform_subformula L n), p.uvars ≤ m → subformula L m n
-| n verum          h := ⊤
-| n (relation r v) h := subformula.relation r (λ i, (v i).to_subterm (by show (v i).uvars ≤ m; simp at h; exact h i))
-| n (imply p q)    h := have h : p.uvars ≤ m ∧ q.uvars ≤ m, by simpa using h, p.to_subformula h.1 ⟶ q.to_subformula h.2
-| n (neg p)        h := ∼p.to_subformula (by simpa using h)
-| n (fal p)        h := ∀'p.to_subformula (by simpa using h)
 
 section encode
 open encodable nat
@@ -202,37 +159,20 @@ namespace subformula
 open uniform_subformula
 variables {L m n}
 
-@[simp] def to_uniform : Π {n}, subformula L m n → uniform_subformula L n
-| n verum          := uniform_subformula.verum
-| n (relation r v) := uniform_subformula.relation r (subterm.to_uniform ∘ v)
-| n (imply p q)    := uniform_subformula.imply p.to_uniform q.to_uniform
-| n (neg p)        := uniform_subformula.neg p.to_uniform
-| n (fal p)        := uniform_subformula.fal p.to_uniform
-
-@[simp] lemma to_uniform_mlift (p : subformula L m n) : p.mlift.to_uniform = p.to_uniform :=
-by simp[mlift]; induction p; simp[mlift', ←fal_eq, ←neg_eq, ←top_eq, ←imply_eq, (∘), *]
-
-@[simp] lemma to_uniform_to_subterm (p : subformula L m n) (h) : p.to_uniform.to_subformula h = p :=
-by induction p; simp*; refl
-
-@[simp] lemma to_subterm_to_uniform (p : uniform_subformula L n) (h : p.uvars ≤ m) : (p.to_subformula h).to_uniform = p :=
-by induction p; simp[←fal_eq, ←neg_eq, ←top_eq, ←imply_eq, (∘), *]
-
 section encode
-
 variables [∀ k, encodable (L.fn k)] [∀ k, encodable (L.pr k)]
 
-def to_nat : subformula L m n → ℕ := λ p, encodable.encode p.to_uniform
+def to_nat : subformula L m n → ℕ := λ p, encodable.encode p.uniform
 
 variables (L m n)
 
 def of_nat : ℕ → option (subformula L m n) := λ i,
   let p := encodable.decode₂ (uniform_subformula L n) i in
-  p.bind (λ p, if h : p.uvars ≤ m then some (p.to_subformula h) else none)
+  p.bind (λ p, if h : p.arity ≤ m then some (p.to_subformula h) else none)
 
 variables {L m n}
 
-@[simp] lemma subformula_uvars (p : subformula L m n) : p.to_uniform.uvars ≤ m :=
+@[simp] lemma subformula_arity (p : subformula L m n) : p.uniform.arity ≤ m :=
 by induction p; simp*
 
 @[simp] lemma to_nat_of_nat (p : subformula L m n) : of_nat L m n p.to_nat = some p :=
@@ -241,7 +181,7 @@ by simp[to_nat, of_nat]
 lemma of_nat_eq_some {e} {p : subformula L m n} : of_nat L m n e = some p ↔ p.to_nat = e :=
 by { simp[of_nat, to_nat, encodable.decode₂_eq_some, dite_eq_iff], split,
   { simp, rintros _ rfl h rfl, simp },
-  { rintros rfl, refine ⟨p.to_uniform, rfl, by simp⟩ } }
+  { rintros rfl, refine ⟨p.uniform, rfl, by simp⟩ } }
 
 @[simp] lemma of_nat_to_nat (p : subformula L m n) : to_nat p.mlift = to_nat p :=
 by simp[to_nat]
