src/QL/FOL/uniform.lean
@@ -1,0 +1,163 @@
+import QL.FOL.semantics
+
+universes u v
+
+namespace fol
+open_locale logic_symbol
+variables (L : language.{u}) {m n : ℕ}
+
+inductive uniform_subterm (n : ℕ) : Type u
+| uvar  {} : ℕ → uniform_subterm
+| var   {} : fin n → uniform_subterm
+| function : ∀ {k}, L.fn k → (fin k → uniform_subterm) → uniform_subterm
+
+@[reducible] def uniform_term := uniform_subterm L 0
+
+inductive uniform_subformula : ℕ → Type u
+| verum    {n} : uniform_subformula n
+| relation {n} : ∀ {p}, L.pr p → (fin p → uniform_subterm L n) → uniform_subformula n
+| imply    {n} : uniform_subformula n → uniform_subformula n → uniform_subformula n
+| neg      {n} : uniform_subformula n → uniform_subformula n
+| fal      {n} : uniform_subformula (n + 1) → uniform_subformula n
+
+prefix `##`:max := uniform_subterm.var
+prefix `&&`:max := uniform_subterm.uvar
+
+namespace uniform_subterm
+variables {L n}
+
+@[simp] def arity : uniform_subterm L n → ℕ
+| &&x            := x + 1
+| ##x            := 0
+| (function f v) := ⨆ᶠ i, (v i).arity
+
+@[simp] def to_subterm : ∀ t : uniform_subterm L n, t.arity ≤ m → subterm L m n
+| &&x                   h := &⟨x, h⟩
+| ##x                   h := #x 
+| (@function L n k f v) h := subterm.function f (λ i, to_subterm (v i) (by { haveI: inhabited (fin k) := ⟨i⟩, simp at h, exact h i}))
+
+section subst
+
+@[simp] def subst (t : uniform_subterm L n) : uniform_subterm L (n + 1) → uniform_subterm L n
+| &&x            := &&x
+| ##x            := (var <* t) x
+| (function f v) := function f (λ i, subst $ v i)
+
+@[simp] def lift : uniform_subterm L n → uniform_subterm L (n + 1)
+| &&x            := &&x
+| ##x            := ##x.succ
+| (function f v) := function f (λ i, (v i).lift)
+
+end subst
+
+section semantics
+variables (S : Structure L) {m} {m₁ m₂ : ℕ} {n} (me : ℕ → S) (e : fin n → S)
+
+@[simp] def val (me : ℕ → S) (e : fin n → S) : uniform_subterm L n → S
+| &&x           := me x
+| ##x           := e x
+| (function f v) := S.fn f (λ i, (v i).val)
+
+@[simp] lemma val_rew (u : uniform_subterm L n) (me : ℕ → S) (e : fin n → S) : ∀ (t : uniform_subterm L (n + 1)),
+  (subst u t).val S me e = t.val S me (e <* val S me e u)
+| &&x            := by simp
+| ##x            := by simp; refine fin.last_cases _ _ x; simp
+| (function f v) := by simp; refine congr_arg _ (by ext i; exact val_rew (v i))
+
+@[simp] lemma val_lift (x : S) (t : uniform_subterm L n) :
+  t.lift.val S me (x *> e) = t.val S me e :=
+by induction t; simp*
+
+end semantics
+
+end uniform_subterm
+
+namespace subterm
+open uniform_subterm
+variables {L m n}
+
+@[simp] def uniform : subterm L m n → uniform_subterm L n
+| &x             := uniform_subterm.uvar x 
+| #x             := uniform_subterm.var x 
+| (function f v) := uniform_subterm.function f (λ i, (v i).uniform)
+
+@[simp] lemma uniform_mlift (t : subterm L m n) : t.mlift.uniform = t.uniform :=
+by induction t; simp*
+
+@[simp] lemma uniform_to_subterm (t : subterm L m n) (h) : t.uniform.to_subterm h = t :=
+by induction t; simp*
+
+@[simp] lemma to_subterm_uniform (t : uniform_subterm L n) (h : t.arity ≤ m) : (t.to_subterm h).uniform = t :=
+by induction t; simp*
+
+@[simp] lemma subterm_arity (t : subterm L m n) : t.uniform.arity ≤ m :=
+by { induction t; simp*, case metavar : i { exact nat.succ_le_iff.mpr i.property } }
+
+section subst
+
+@[simp] lemma uniform_subst (u : subterm L m n) (t : subterm L m (n + 1)) :
+  (subst u t).uniform = uniform_subterm.subst u.uniform t.uniform :=
+by { induction t; simp*, case var : x { refine fin.last_cases _ _ x; simp } }
+
+@[simp] lemma uniform_push (t : subterm L m (n + 1)) :
+  (push t).uniform = uniform_subterm.subst (&&m) t.uniform :=
+by { induction t; simp*, case var : x { refine fin.last_cases _ _ x; simp } }
+
+lemma uniform_lift (t : subterm L m n) :
+  t.lift.uniform = t.uniform.lift :=
+by induction t; simp*
+
+end subst
+
+section semantics
+variables (S : Structure L) {m} {m₁ m₂ : ℕ} {n} (me : ℕ → S) (e : fin n → S)
+
+@[simp] lemma uniform_val (t : subterm L m n) : t.uniform.val S me e = t.val S (λ i, me i) e :=
+by induction t; simp*
+
+end semantics
+
+end subterm
+
+namespace uniform_subformula
+variables {L n}
+
+@[simp] def arity : Π {n}, uniform_subformula L n → ℕ
+| n verum          := 0
+| n (relation r v) := ⨆ᶠ i, (v i).arity
+| n (imply p q)    := max p.arity q.arity
+| n (neg p)        := p.arity
+| n (fal p)        := p.arity
+
+@[simp] def to_subformula : ∀ {n} (p : uniform_subformula L n), p.arity ≤ m → subformula L m n
+| n verum          h := ⊤
+| n (relation r v) h := subformula.relation r (λ i, (v i).to_subterm (by show (v i).arity ≤ m; simp at h; exact h i))
+| n (imply p q)    h := have h : p.arity ≤ m ∧ q.arity ≤ m, by simpa using h, p.to_subformula h.1 ⟶ q.to_subformula h.2
+| n (neg p)        h := ∼p.to_subformula (by simpa using h)
+| n (fal p)        h := ∀'p.to_subformula (by simpa using h)
+
+end uniform_subformula
+
+namespace subformula
+open uniform_subformula
+variables {L m n}
+
+@[simp] def uniform : Π {n}, subformula L m n → uniform_subformula L n
+| n verum          := uniform_subformula.verum
+| n (relation r v) := uniform_subformula.relation r (subterm.uniform ∘ v)
+| n (imply p q)    := uniform_subformula.imply p.uniform q.uniform
+| n (neg p)        := uniform_subformula.neg p.uniform
+| n (fal p)        := uniform_subformula.fal p.uniform
+
+@[simp] lemma uniform_mlift (p : subformula L m n) : p.mlift.uniform = p.uniform :=
+by simp[mlift]; induction p; simp[mlift', ←fal_eq, ←neg_eq, ←top_eq, ←imply_eq, (∘), *]
+
+@[simp] lemma uniform_to_subterm (p : subformula L m n) (h) : p.uniform.to_subformula h = p :=
+by induction p; simp*; refl
+
+@[simp] lemma to_subterm_uniform (p : uniform_subformula L n) (h : p.arity ≤ m) : (p.to_subformula h).uniform = p :=
+by induction p; simp[←fal_eq, ←neg_eq, ←top_eq, ←imply_eq, (∘), *]
+
+end subformula
+
+end fol
